DependentComputability/OmegaPart.lean
@@ -1,0 +1,222 @@
+import DependentComputability.Tactic.RecursorModel
+
+-- Credit to Anthony Vandikas for the idea of `ωPart` (YellPika on github)
+
+@[elab_as_elim]
+def Nat.geRec {n : ℕ} {motive : ∀ m ≤ n, Sort u}
+    (refl : motive n le_rfl) (step : ∀ m, (h : m < n) → motive (m + 1) h → motive m (le_of_lt h))
+    {m : ℕ} (t : m ≤ n) : motive m t :=
+  if h : m < n then
+    step m h (Nat.geRec refl step h)
+  else
+    Nat.le_antisymm t (Nat.not_lt.mp h) ▸ refl
+termination_by n - m
+decreasing_by exact sub_succ_lt_self n m h
+
+structure ωProp where
+  toFun : ℕ → Bool
+
+namespace ωProp
+
+@[coe]
+def coe (x : ωProp) : Prop :=
+  ∃ y, x.toFun y
+
+instance : CoeSort ωProp Prop where
+  coe := ωProp.coe
+
+protected def false : ωProp := .mk fun _ => false
+protected def true : ωProp := .mk fun _ => true
+
+@[simp] theorem coe_mk (f : ℕ → Bool) : mk f ↔ ∃ n, f n := by simp [coe]
+@[simp] theorem coe_false : ωProp.false ↔ False := by simp [ωProp.false]
+@[simp] theorem coe_true : ωProp.true ↔ True := by simp [ωProp.true]
+
+def bind (p : ωProp) (f : p → ωProp) : ωProp where
+  toFun n := go n 0
+where
+  go (fuel : ℕ) (n : ℕ) : Bool :=
+    match fuel with
+    | 0 => false
+    | fuel + 1 =>
+      if h : p.toFun n then
+        (f ⟨n, h⟩).toFun fuel
+      else
+        go fuel (n + 1)
+
+@[simp] theorem coe_bind {p : ωProp} {f : p → ωProp} :
+    bind p f ↔ ∃ h : p, f h := by
+  simp only [bind, coe_mk]
+  constructor
+  · intro ⟨fuel, hfuel⟩
+    generalize 0 = n at hfuel
+    fun_induction bind.go with
+    | case1 => contradiction
+    | case2 n fuel hp => exact ⟨⟨n, hp⟩, ⟨fuel, hfuel⟩⟩
+    | case3 n fuel hp ih => exact ih hfuel
+  · rintro ⟨⟨n, hp⟩, ⟨m, hf⟩⟩
+    let +generalize n' := 0
+    have hn' : n' ≤ n := n.zero_le
+    clear_value n'
+    induction hn' using Nat.geRec with
+    | refl => use m + 1; simp [bind.go, hp, hf]
+    | step n' hn' ih =>
+      by_cases hp : p.toFun n'
+      · use m + 1; simp [bind.go, hp, hf]
+      · obtain ⟨fuel, hfuel⟩ := ih
+        use fuel + 1; simp [bind.go, hp, hfuel]
+
+-- ∃ n, ∃ h : ∀ k ≤ n, dom k, p n (h .rfl) = true
+def rfind (dom : ℕ → ωProp) (p : ∀ n, dom n → Bool) : ωProp where
+  toFun n := go n 0 0
+where
+  go (fuel : ℕ) (n k : ℕ) : Bool :=
+    match fuel with
+    | 0 => false
+    | fuel + 1 =>
+      if h : (dom n).toFun k then
+        if p n ⟨k, h⟩ then
+          true
+        else
+          go fuel (n + 1) 0
+      else
+        go fuel n (k + 1)
+
+@[simp] theorem coe_rfind {dom : ℕ → ωProp} {p : ∀ n, dom n → Bool} :
+    rfind dom p ↔ ∃ n, (∃ h : dom n, p n h) ∧ ∀ k < n, dom k := by
+  simp only [rfind, coe_mk]
+  constructor
+  · intro ⟨fuel, hfuel⟩
+    let n := 0; let k := 0
+    change rfind.go dom p fuel n k at hfuel
+    have hn : ∀ m < n, dom m := by simp [n]
+    clear_value n k
+    fun_induction rfind.go with
+    | case1 => contradiction
+    | case2 n k fuel hk hp => exact ⟨n, ⟨⟨k, hk⟩, hp⟩, hn⟩
+    | case3 n k fuel hk hp ih =>
+      refine ih hfuel ?_
+      intro m hm
+      rw [Nat.lt_add_one_iff_lt_or_eq] at hm
+      rcases hm with hm | rfl
+      · exact hn m hm
+      · exact ⟨k, hk⟩
+    | case4 n k fuel hk ih => exact ih hfuel hn
+  · rintro ⟨n, ⟨⟨k, hk⟩, hp⟩, hn⟩
+    let n' := 0; let k' := 0
+    change ∃ fuel, rfind.go dom p fuel n' k'
+    have hn' : n' ≤ n := Nat.zero_le n
+    have hk'₁ (hn' : n' < n) : ∃ m, (dom n').toFun m ∧ k' ≤ m := by
+      obtain ⟨m, hm⟩ := hn n' hn'
+      exact ⟨m, hm, m.zero_le⟩
+    have hk'₂ : n' = n → k' ≤ k := fun _ => Nat.zero_le k
+    clear_value n' k'
+    induction hn' using Nat.geRec generalizing k' with
+    | refl =>
+      specialize hk'₂ rfl; clear hk'₁
+      induction hk'₂ using Nat.geRec with
+      | refl => use 1; simp [rfind.go, hk, hp]
+      | @step k' hk' ih =>
+        obtain ⟨fuel, hfuel⟩ := ih
+        use fuel + 1; rw [rfind.go]
+        split
+        · rfl
+        · assumption
+    | @step n' hn' ih =>
+      specialize ih 0 (fun hn' => ?_) (fun _ => k.zero_le)
+      · obtain ⟨m, hm⟩ := hn (n' + 1) hn'
+        exact ⟨m, hm, m.zero_le⟩
+      obtain ⟨fuel, hfuel⟩ := ih
+      obtain ⟨m, hm, hm'⟩ := hk'₁ hn'
+      clear hk'₁ hk'₂
+      induction hm' using Nat.geRec with
+      | refl => use fuel + 1; simp [rfind.go, hm, hfuel]
+      | @step k' hk' ih =>
+        obtain ⟨fuel', hfuel'⟩ := ih
+        by_cases hdom : (dom n').toFun k'
+        · use fuel + 1; simp [rfind.go, hfuel, hdom]
+        · use fuel' + 1; simp [rfind.go, hfuel', hdom]
+
+end ωProp
+
+structure ωPart (α : Sort u) where
+  Dom : ωProp
+  get : Dom → α
+
+@[coe]
+def ωPart.coe (x : ωPart α) : Part α where
+  Dom := x.Dom
+  get := x.get
+
+instance : Coe (ωPart α) (Part α) where
+  coe := ωPart.coe
+
+protected def ωPart.pure (x : α) : ωPart α where
+  Dom := .true
+  get _ := x
+
+protected def ωPart.bind (x : ωPart α) (f : α → ωPart β) : ωPart β where
+  Dom := .bind x.Dom (fun h => (f (x.get h)).Dom)
+  get h := (f (x.get (ωProp.coe_bind.mp h).1)).get (ωProp.coe_bind.mp h).2
+
+def ωPart.rfind (p : ℕ → ωPart Bool) : ωPart ℕ where
+  Dom := .rfind (fun n => (p n).Dom) (fun n => (p n).get)
+  get h := Nat.rfindX (fun n => p n) (by simpa using h)
+
+@[simp]
+theorem ωPart.coe_pure (x : α) :
+    (ωPart.pure x : Part α) = Part.some x := by
+  apply Part.ext' <;> simp [ωPart.coe, ωPart.pure]
+
+@[simp]
+theorem ωPart.coe_bind (x : ωPart α) (f : α → ωPart β) :
+    (x.bind f : Part β) = Part.bind x (fun y => f y) := by
+  apply Part.ext' <;> simp [ωPart.coe, ωPart.bind, Part.bind, Part.assert]
+
+@[simp]
+theorem ωPart.coe_rfind (p : ℕ → ωPart Bool) :
+    (rfind p : Part ℕ) = Nat.rfind (fun n => p n) := by
+  apply Part.ext' <;> simp [ωPart.coe, ωPart.rfind, Nat.rfind]
+
+set_option Elab.async false in
+set_option linter.unusedVariables false in
+theorem Nat.Partrec.exists_ωPart_eq {f : ℕ →. ℕ} (hf : Nat.Partrec f) :
+    ∃ g : ℕ → ωPart ℕ, ∃ g' : new_type% g, ∃ h : DComp g, ∃ h' : new_type% h, ∀ n, f n = g n := by
+  induction hf with
+  | zero =>
+    use fun _ => .pure 0, new% _, by other_dcomp_tac, new% _
+    simp [pure, PFun.pure]
+  | succ =>
+    use fun n => .pure (n + 1), new% _, by other_dcomp_tac, new% _
+    simp
+  | left =>
+    use fun n => .pure n.unpair.1, new% _, by other_dcomp_tac, new% _
+    simp
+  | right =>
+    use fun n => .pure n.unpair.2, new% _, by other_dcomp_tac, new% _
+    simp
+  | @pair f g hf hg fih gih =>
+    obtain ⟨gf, gf', hgf, hgf', hgf''⟩ := fih
+    obtain ⟨gg, gg', hgg, hgg', hgg''⟩ := gih
+    use fun n => (gf n).bind fun a => (gg n).bind fun b => .pure (Nat.pair a b)
+    use new% _, by other_dcomp_tac, new% _
+    simp [Seq.seq, hgf'', hgg'', Part.bind_some_eq_map]
+  | @comp f g hf hg fih gih =>
+    obtain ⟨gf, gf', hgf, hgf', hgf''⟩ := fih
+    obtain ⟨gg, gg', hgg, hgg', hgg''⟩ := gih
+    use fun n => (gg n).bind fun m => gf m
+    use new% _, by other_dcomp_tac, new% _
+    simp [← hgf'', hgg'']
+  | @prec f g hf hg fih gih =>
+    obtain ⟨gf, gf', hgf, hgf', hgf''⟩ := fih
+    obtain ⟨gg, gg', hgg, hgg', hgg''⟩ := gih
+    use (unpaired fun a n => n.rec (gf a) fun y IH => IH.bind fun i => gg (a.pair (y.pair i)))
+    use new% _, by other_dcomp_tac, new% _
+    intro n
+    simp only [unpaired, Part.bind_eq_bind]
+    induction (unpair n).2 <;> simp_all
+  | @rfind f hf ih =>
+    obtain ⟨g, g', hg, hg', hg''⟩ := ih
+    use fun a => .rfind fun n => (g (a.pair n)).bind fun m => .pure (m = 0)
+    use new% _, by other_dcomp_tac, new% _
+    simp [hg'', Part.bind_some_eq_map]
